theories/examples_wp.v
@@ -1,95 +1,18 @@
-Require Import base lang free eval step wp encode.
-
 From iris.proofmode Require Import base proofmode classes.
-
 From iris.base_logic.lib Require Import fancy_updates.
 From iris.bi Require Import weakestpre.
 From iris.prelude Require Import options.
 Import uPred.
 
-Require Import wp.
+Require Import base lang free eval step wp wp_tactics encode.
+
+
 Context `{!osirisGS_gen hlc Σ}.
 
 
-(* ---------------------------------------------------------------------- *)
-(* Tactics to work on WPs. They mimic those on [is_safe]. *)
-
-(* TODO:
- * - instead of using [cbn], try to only reduce what should be reduced (not continutations, ...).
- * - eliminate later modalities if required.
- *   It can *at least* be done when the goal is automatically provable after 
- *   [repeat iNext].
- * - move the tactics and tactics-related elements to a new file [theories/wp_tactics.v]
- *)
-
-Definition our__id {A}: A → A := λ i, i.
-Lemma our__id_is_id {A} (i: A) :
-  i = our__id i.
-Proof. reflexivity. Qed.
-Global Opaque our__id.
-
-Ltac wp_step :=
-  lazymatch goal with
-  | |- environments.envs_entails _
-        (wp _ _ (ret _) _) => iApply wp_ret
-  | |- environments.envs_entails _
-        (wp _ _ (bind _ _) _) => iApply wp_bind
-  | |- environments.envs_entails _
-        (wp _ _ (Par (ret _) (ret _) _ _) _) => iApply wp_par_ret_ret
-  | |- environments.envs_entails _
-        (wp _ _ (Par _ (ret _) ?k ?ko) _) =>
-      remember k; remember ko;
-      iApply wp_par_ret_right
-  | |- environments.envs_entails _
-        (wp _ _ (Par (ret _) _ ?k ?ko) _) =>
-      remember k; remember ko;
-      iApply wp_par_ret_left
-  | |- environments.envs_entails _
-        (wp _ _ (try (ret _) _ _) _) => iApply wp_try_ret
-  | |- environments.envs_entails _
-        (wp _ _ (eval.lookup _ _) _) => simpl (eval.lookup _ _)
-  | H: ?k = _ |- environments.envs_entails _
-        (wp _ _ (?k _) _) =>
-      rewrite H; clear H k
-  end;
-  cbn.
-
-Ltac wp :=
-  cbn;
-  repeat
-    lazymatch goal with
-    | |- environments.envs_entails _ (bi_later _) => iNext
-    | _ => wp_step
-    end.
-
-Ltac wp_par :=
-  iApply wp_par; [wp | wp | ].
-
-Ltac wp_par_with H :=
-  iApply (wp_par with H); [wp | wp | ].
-
-Ltac wp_use H :=
-  first [
-    iApply H
-  | iApply wp_covariant; [ iApply H |]
-  ];
-  simpl.
-
-Global Opaque call.
-Ltac wp_call :=
-  with_strategy transparent [call] unfold call at 1; wp.
 
 
-(* TODO not great *)
-Ltac wp_set_postcondition :=
-  match goal with
-    |- @environments.envs_entails _ _
-        (?ϕ ?v) =>
-      is_evar ϕ;
-      instantiate (1 := (λ w, ⌜w = v⌝)%I)
-  end.
-
-(* ----------------------------------------------------------------------*)
+(* ---------------------------------------------------------------------------*)
 (* Examples. *)
 
 
@@ -106,26 +29,26 @@ Proof.
 Abort. (* expected *)
 
 (* let x = (A (), B ()) in let (x1, x2) = x in x1 *)
-
 Definition example :=
   ELet1Var "x" (EPair (EConstant "A") (EConstant "B")) $
-  ELet1 (PPair (PVar "x1") (PVar "x2")) (EVar "x") $
-  EVar "x1".
+    ELet1 (PPair (PVar "x1") (PVar "x2")) (EVar "x") $
+    EVar "x1".
+
 
 (* An example of reasoning about straight-line code. *)
 
 Goal
   ⊢ WP (eval EnvNil example) {{ λ v, ⌜v = VData "A" (VTuple VNil)⌝ }}.
 Proof.
-  iStartProof. by wp.
+  by wp.
 Qed.
 
 (* let x = (z1, z2) in let (x1, x2) = x in x1 *)
 
 Definition example2 :=
   ELet1Var "x" (EPair (EVar "z1") (EVar "z2")) $
-  ELet1 (PPair (PVar "x1") (PVar "x2")) (EVar "x") $
-  EVar "x1".
+    ELet1 (PPair (PVar "x1") (PVar "x2")) (EVar "x") $
+    EVar "x1".
 
 Goal
   ∀ v1 v2,
@@ -142,17 +65,18 @@ Definition example3 :=
   EPair idA idA.
 
 (* TODO. *)
-Lemma spec_example3:
+Lemma spec_example3 s E:
   ∀ (id : val),
-  ⊢ □ (∀ v, WP (call id v) {{λ v', ⌜ v' = v⌝ }} ) -∗
+  ⊢ □ (∀ v, WP (call id v) @ s; E {{λ v', ⌜ v' = v⌝ }} ) -∗
   let env := EnvCons "id" id EnvNil in
-  WP (eval env example3) {{λ v, ⌜v = VPair (VConstant "A") (VConstant "A")⌝ }}.
+  WP (eval env example3) @ s; E
+                                {{λ v, ⌜v = VPair (VConstant "A") (VConstant "A")⌝ }}.
 Proof.
   iIntros (id) "#Hid".
   wp.
-  (* The two components of the pair are evaluated in parallel,
-     and each of them is a function application, which is itself
-     evaluated in parallel. So we have a tree of nested [Par]. *)
+  (* The two components of the pair are evaluated in parallel, and each of them 
+   * is a function application, which is itself evaluated in parallel. So we 
+   * have a tree of nested [Par]. *)
   wp_par.
   { iApply "Hid". }
   { iApply wp_covariant.
@@ -167,19 +91,20 @@ Qed.
 
 (* The identity function. *)
 
-(* [identity] is an expression which returns a closure whose behavior is
-   the identity function. *)
+(* [identity] is an expression which returns a closure whose behavior is the 
+ * identity function. *)
 
 Definition identity :=
   EFun "x" (EVar "x").
 
 Lemma spec_identity s E:
-  ⊢ □ WP (eval EnvNil identity) @ s; E {{λ c, ∀ v, WP (call c v) @ s; E {{ λ v', ⌜v' = v⌝ }} }}.
+  ⊢ □ WP (eval EnvNil identity) @ s; E
+                                       {{λ c, □ ∀ v, WP (call c v) @ s; E {{ λ v', ⌜v' = v⌝ }} }}.
 Proof.
   iModIntro.
-  wp. iIntros.
-  Admitted.
-  (*by wp_call.
+  wp.
+  iModIntro. iIntros.
+  by wp_call.
 Qed.
 
 (* let id = identity in
@@ -187,10 +112,11 @@ Qed.
 
 Definition example4 :=
   ELet1Var "id" identity $
-  example3.
+    example3.
 
 Lemma spec_example4 s E:
-  ⊢ WP (eval EnvNil example4) @ s; E {{λ v, ⌜v = VPair (VConstant "A") (VConstant "A")⌝ }}.
+  ⊢ WP (eval EnvNil example4) @ s; E
+                                     {{λ v, ⌜v = VPair (VConstant "A") (VConstant "A")⌝ }}.
 Proof.
   unfold example4.
   (* Abstract away the [identity] function; its spec suffices. *)
@@ -200,31 +126,27 @@ Proof.
   generalize example3 spec_example3.
   intros example3 Hexample3.
   (* Attack the goal. *)
+  iStartProof.
   wp.
-  iPoseProof (Hidentity s E) as "#Hid".
-  wp_par.
-  - wp_use "Hid".
-  - wp.
-    iNext. wp_set_postcondition.
-    iPureIntro. reflexivity.
-  - iNext.
-    iIntros (v1 v2) "H->". wp.
-Admitted.
+  wp_use Hidentity.
+  iIntros (id) "#Hid". wp.
+  by wp_use Hexample3.
+Qed.
 
-(*
 (* An example that involves an assertion. *)
 
 Definition example5 :=
   ESeq (EAssert ETrue) EFalse.
 
-Lemma spec_example5:
-  wp EnvNil example5 (λ v, v = VFalse).
+Lemma spec_example5 s E:
+  ⊢ WP (eval EnvNil example5) @ s; E {{ λ v, ⌜v = VFalse⌝ }}.
 Proof.
   wp.
+  iIntros ([|]).
   (* Subgoal: prove that [assert true] succeeds. *)
-  { reflexivity. }
+  { by wp. }
   (* Remainder: prove that [false] returns [false], as promised. *)
-  reflexivity.
+  by wp.
 Qed.
 
 (* let id = identity in
@@ -232,11 +154,11 @@ Qed.
 
 Definition example4b :=
   ELet1Var "id" identity $
-  let id := EVar "id" in
-  EApp (EApp id id) EUnit.
+    let id := EVar "id" in
+    EApp (EApp id id) EUnit.
 
-Lemma spec_example4b:
-  wp EnvNil example4b (λ v, v = VUnit).
+Lemma spec_example4b s E:
+  ⊢ WP (eval EnvNil example4b) @ s; E {{λ v, ⌜v = VUnit⌝ }}.
 Proof.
   unfold example4b.
   (* Abstract away the [identity] function; its spec suffices. *)
@@ -246,11 +168,12 @@ Proof.
   wp.
   (* Exploit the spec of the expression [identity]. *)
   wp_use Hidentity.
-  revert a H; intros id Hid. (* TODO wp_intros does not let us pick names *)
+  iIntros (id) "#Hid".
   wp.
   (* We are looking at [id id]. *)
-  wp_use Hid.
-  wp_use Hid.
+  wp_use "Hid".
+  iIntros(?->).
+  wp_use "Hid".
 Qed.
 
 (* let id = identity in
@@ -258,11 +181,11 @@ Qed.
 
 Definition example4c :=
   ELet1Var "id" identity $
-  let id := EVar "id" in
-  EApp id (EApp id EUnit).
+    let id := EVar "id" in
+    EApp id (EApp id EUnit).
 
-Lemma spec_example4c:
-  wp EnvNil example4c (λ v, v = VUnit).
+Lemma spec_example4c s E:
+  ⊢ WP (eval EnvNil example4c) @ s; E {{λ v, ⌜v = VUnit⌝}}.
 Proof.
   unfold example4c.
   (* Abstract away the [identity] function; its spec suffices. *)
@@ -272,11 +195,12 @@ Proof.
   wp.
   (* Exploit the spec of the expression [identity]. *)
   wp_use Hidentity.
-  revert a H; intros id Hid. (* TODO wp_intros does not let us pick names *)
+  iIntros (id) "#Hid".
   wp.
   (* We are looking at [id()]. *)
-  wp_use Hid.
-  wp_use Hid.
+  wp_use "Hid".
+  iIntros(?->).
+  wp_use "Hid".
 Qed.
 
 (* let id = identity in
@@ -284,11 +208,11 @@ Qed.
 
 Definition example4d :=
   ELet1Var "id" identity $
-  let id := EVar "id" in
-  EApp (EApp id id) (EApp id EUnit).
+    let id := EVar "id" in
+    EApp (EApp id id) (EApp id EUnit).
 
-Lemma spec_example4d:
-  wp EnvNil example4d (λ v, v = VUnit).
+Lemma spec_example4d s E:
+  ⊢ WP (eval EnvNil example4d) @ s; E {{λ v, ⌜v = VUnit⌝}}.
 Proof.
   unfold example4d.
   (* Abstract away the [identity] function; its spec suffices. *)
@@ -298,59 +222,66 @@ Proof.
   wp.
   (* Exploit the spec of the expression [identity]. *)
   wp_use Hidentity.
-  revert a H; intros id Hid. (* TODO wp_intros does not let us pick names *)
-  (* Here, [wp] is unable to make progress because we are looking at two
-     function calls in parallel. *)
+  iIntros (id) "#Hid".
+
+  (* We currently need [wp_restore] here to get the continuation that was stored 
+   * in a hypotheses. *)
+  wp_restore.
   wp_par.
 
   (* id id *)
-  { wp_use Hid. }
+  { wp_use "Hid". }
 
   (* id () *)
-  { wp_use Hid. }
+  { wp_use "Hid". }
 
-  wp_intros.
-  wp_use Hid.
+  iIntros (??->->).
+  wp_use "Hid".
 Qed.
 
 (* let rec diverge x = diverge x in diverge() *)
 
 Definition divergence :=
   ELetRec1 "diverge" "x" (EApp (EVar "diverge") (EVar "x")) $
-  EApp (EVar "diverge") EUnit.
+    EApp (EVar "diverge") EUnit.
 
 Lemma spec_divergence:
-  wp EnvNil divergence (λ _, False).
+  ⊢ WP (eval EnvNil divergence) {{λ _, ⌜False⌝}}.
 Proof.
-  (* The tactic [wp_step] can be applied as many times as one wishes,
+  (* The tactic [wp_call] can be applied as many times as one wishes,
      since this term does not terminate, but the goal can never be
-     reached in this way. *)
-  do 100 wp_step.
-Abort. (* TODO once we have Löb induction, prove this goal *)
+     reached in this way.
+     TODO: reduce the gap between the tactics in [safe_*] and those in [wp_*] in
+     order to use [wp_step] below. *)
+  wp.
+  Time do 100 wp_call.
+
+Abort. (* TODO now that we have Löb induction, prove this goal *)
 
 (* -------------------------------------------------------------------------- *)
 
 (* A recursive function that walks a list. *)
 
 (* let rec walk xs =
-     match xs with
-     | [] -> ()
-     | x :: xs -> walk xs *)
+   match xs with
+   | [] -> ()
+   | x :: xs -> walk xs *)
 
 Definition walk : rec_bindings :=
   RecBinding1 "walk" "xs" (
-    EMatch (EVar "xs") (
-      BrCons (Branch pNil EUnit) $
-      BrCons (Branch (pCons (PVar "x") (PVar "xs"))
-                     (EApp (EVar "walk") (EVar "xs"))
-             ) $
-      BrNil
-    )
-  ).
+      EMatch (EVar "xs") (
+          BrCons (Branch pNil EUnit) $
+            BrCons (Branch (pCons (PVar "x") (PVar "xs"))
+                      (EApp (EVar "walk") (EVar "xs"))
+            ) $
+            BrNil
+        )
+    ).
 
-Lemma spec_walk :
+Lemma spec_walk s E:
   ∀ (bs : list bool) η,
-  safe (call (VCloRec η walk "walk") (encode_list bs)) (λ v, v = VUnit).
+  ⊢ WP (call (VCloRec η walk "walk") (encode_list bs)) @s; E
+                                                             {{λ v, ⌜v = VUnit⌝}}.
 Proof.
   (* The environment that is captured by the closure does not matter,
      since the code is in fact closed. So, we must in fact universally
@@ -360,62 +291,66 @@ Proof.
      the semantics. Instead we would like to refer this value as "the
      value produced by evaluating the recursive bindings [walk]". *)
   induction bs as [| b bs ]; intro η; wp_call.
-  { reflexivity. }
+  { iPureIntro. reflexivity. }
   { wp_use IHbs. }
 Qed.
 
 Definition walk_example e :=
   ELetRec walk $
-  EApp (EVar "walk") e.
+    EApp (EVar "walk") e.
 
-Lemma spec_walk_example_concrete :
-  let e := (eCons ETrue (eCons EFalse eNil)) in
-  wp EnvNil (walk_example e) (λ v, v = encode ()).
-Proof.
-  (* The code is pure and terminating and can be fully evaluated. *)
-  wp. do 3 wp_call. reflexivity.
-Qed.
+(* TODO: resolve evar-related issues.
 
-Lemma spec_walk_example_abstract :
-  forall (bs : list bool),
-  let η := EnvCons "xs" (encode bs) EnvNil in
-  wp η (walk_example (EVar "xs")) (λ v, v = encode ()).
-Proof.
-  intros. wp. wp_use spec_walk.
-Qed.
+   Lemma spec_walk_example_concrete s E:
+   let e := (eCons ETrue (eCons EFalse eNil)) in
+   ⊢ WP (eval EnvNil (walk_example e)) @ s; E {{λ v, ⌜v = encode ()⌝}}.
+   Proof.
+     (* The code is pure and terminating and can be fully evaluated. *)
+   wp. do 3 wp_call. reflexivity.
+   Qed.
 
-(* -------------------------------------------------------------------------- *)
+   Lemma spec_walk_example_abstract s E:
+   forall (bs : list bool),
+   let η := EnvCons "xs" (encode bs) EnvNil in
+   ⊢ WP (eval η (walk_example (EVar "xs"))) @ s; E {{ λ v, ⌜v = encode ()⌝ }}.
+   Proof.
+   intros. wp. wp_use spec_walk.
+   Qed. *)
+
+(* ------------------------------------------------------------------------- *)
 
 (* A recursive function that computes the length of a list. *)
 
 (* let rec length xs =
-     match xs with
-     | [] -> 0
-     | x :: xs -> 1 + length xs *)
+    match xs with
+    | [] -> 0
+    | x :: xs -> 1 + length xs *)
 
 Definition length : rec_bindings :=
   RecBinding1 "length" "xs" (
-    EMatch (EVar "xs") (
-      BrCons (Branch pNil (EInt 0)) $
-      BrCons (Branch (pCons (PVar "x") (PVar "xs"))
-                     (EIntAdd (EInt 1) (EApp (EVar "length") (EVar "xs")))
-             ) $
-      BrNil
-    )
-  ).
+      EMatch (EVar "xs") (
+          BrCons (Branch pNil (EInt 0)) $
+            BrCons (Branch (pCons (PVar "x") (PVar "xs"))
+                      (EIntAdd (EInt 1) (EApp (EVar "length") (EVar "xs")))
+            ) $
+            BrNil
+        )
+    ).
 
-Lemma spec_length :
+Lemma spec_length s E :
   ∀ `{Encode A} (xs : list A) η,
-  safe
-    (call (VCloRec η length "length") (encode_list xs))
-    (λ v, v = encode (List.length xs)).
+  ⊢ WP
+      (call (VCloRec η length "length") (encode_list xs))
+      @ s; E
+             {{ λ v, ⌜v = encode (List.length xs)⌝ }}.
 Proof.
   induction xs as [| x xs ]; intro η; wp_call.
-  { reflexivity. }
+  { iPureIntro. reflexivity. }
   { wp_use IHxs. wp.
     rewrite Nat2Z.inj_succ.
+    iIntros(?->).
+    wp.
+    iPureIntro.
     rewrite int.add_repr_repr.
     do 2 f_equal. lia. }
 Qed.
-
-*) *)
