theories/wp_tactics.v
@@ -1,0 +1,108 @@
+From iris.proofmode Require Import proofmode.
+From iris.bi Require Import weakestpre.
+Require Import free eval wp.
+
+(* ---------------------------------------------------------------------- *)
+(* Tactics to work on WPs. They mimic those on [is_safe]. *)
+
+(* TODO:
+ * - instead of using [cbn], try to only reduce what should be reduced
+ *   For example, continuations and hypotheses should never be reduced by
+ *   tactics aimed for the goal.
+ *
+ * - Find a better way to hide continuations.
+ *   The current behaviour is:
+ *     if the goal is a [Par _ ret k ko] or [Par ret _ k ko], then remember
+ *     [k] and [ko].
+ *   Thus, continuations only appear once in the proof term as the other
+ *   occurences are replaced by the fresh variable allocated by [remember].
+ *
+ *   This is important, as it prevents the proof term (and the duration
+ *   of lemmas applications and Qed) to explode
+ *
+ *   Note : the use of an ad-hoc opaque identity function is also slow.
+ *          => TODO: understand why and if fixable, use it instead.
+ *)
+
+Ltac wp_restore :=
+  try lazymatch goal with
+    | H: ?k = _ |- environments.envs_entails _
+                    (wp _ _ (?k _) _) =>
+        rewrite H (* -our__id_is_id *); clear H k
+    end.
+
+Ltac wp_remember k :=
+  let Hk := fresh "Hk" in
+  remember k eqn:Hk.
+
+Ltac wp_step :=
+  wp_restore;
+  (* The lazymatch stills misses a few cases and should be completed. *)
+  lazymatch goal with
+  | |- environments.envs_entails _
+        (wp _ _ (ret _) _) => iApply wp_ret
+  | |- environments.envs_entails _
+        (wp _ _ (bind _ _) _) => iApply wp_bind
+  | |- environments.envs_entails _
+        (wp _ _ (Par (ret _) (ret _) _ _) _) => iApply wp_par_ret_ret
+  | |- environments.envs_entails _
+        (wp _ _ (Par _ (ret _) ?k ?ko) _) =>
+      wp_remember k;
+      wp_remember ko;
+      iApply wp_par_ret_right
+  | |- environments.envs_entails _
+        (wp _ _ (Par (ret _) _ ?k ?ko) _) =>
+      wp_remember k;
+      wp_remember ko;
+      iApply wp_par_ret_left
+  | |- environments.envs_entails _
+        (wp _ _ (try (ret _) _ _) _) => iApply wp_try_ret
+  | |- environments.envs_entails _
+        (wp _ _ (eval.lookup _ _) _) => simpl (eval.lookup _ _)
+  | |- environments.envs_entails _
+        (wp _ _ (stop Eval _) _) =>
+      (iApply wp_eval_ret + iApply wp_eval)
+  | |- environments.envs_entails _
+        (wp _ _ (Stop Flip _ _) _) => iApply wp_flip
+  | H: ?k = _ |- environments.envs_entails _
+                  (wp _ _ (?k _) _) =>
+      rewrite H; clear H k
+  end;
+  cbn.
+
+Ltac wp :=
+  iStartProof;
+  cbn; (* TODO: better control the reduction strategy. *)
+  (repeat
+    lazymatch goal with
+    | |- environments.envs_entails _ (bi_later _) => iNext
+    | _ => wp_step
+     end);
+  repeat wp_restore.
+
+Ltac wp_par :=
+  iApply wp_par; [wp | wp | ]; wp_restore.
+
+Ltac wp_par_with H :=
+  iApply (wp_par with H); [wp | wp | ]; wp_restore.
+
+Ltac wp_use H :=
+  first [
+    iApply H
+  | iApply wp_covariant; [ iApply H |]
+  ];
+  simpl; wp_restore.
+
+Global Opaque call.
+Ltac wp_call :=
+  with_strategy transparent [call] unfold call; wp.
+
+
+(* TODO not great *)
+Ltac wp_set_postcondition :=
+  match goal with
+    |- @environments.envs_entails _ _
+        (?ϕ ?v) =>
+      is_evar ϕ;
+      instantiate (1 := (λ w, ⌜w = v⌝)%I)
+  end.
